Clean/Gadgets/Keccak/Theta.lean
@@ -16,7 +16,6 @@ def theta (state : Var KeccakState (F p)) : Circuit (F p) (Var KeccakState (F p)
 instance elaborated : ElaboratedCircuit (F p) KeccakState KeccakState where
   main := theta
   local_length _ := 480
-  output _ i0 := var_from_offset KeccakState (i0 + 280)
 
 def assumptions (state : KeccakState (F p)) := state.is_normalized
 
